Ctx

Qdt/MLTT/Context.lean
@@ -3,39 +3,41 @@ import Qdt.Tele
 
 namespace Qdt
 
-abbrev Ctx := Tele Param
+namespace Ctx
 
-def Ctx.get {n} : Idx n → Ctx 0 n → Ty n
+def get {n} : Idx n → Ctx 0 n → Ty n
   | i, .nil => nomatch i
   | ⟨0, _⟩, .snoc _ ⟨_, _, A⟩ => ↑A
-  | ⟨i + 1, hi⟩, .snoc Γ _ => ↑Ctx.get ⟨i, Nat.lt_of_succ_lt_succ hi⟩ Γ
+  | ⟨i + 1, hi⟩, .snoc Γ _ => ↑get ⟨i, Nat.lt_of_succ_lt_succ hi⟩ Γ
 
-def Ctx.weaken {a b} : Ctx a b → Ctx (a + 1) (b + 1) :=
+def weaken {a b} : Ctx a b → Ctx (a + 1) (b + 1) :=
   Tele.dmap 1 (fun ⟨src, x, t⟩ => ⟨src, x, t.subst Subst.shift⟩)
 
 @[simp]
-theorem Ctx.weaken_nil {n} : Ctx.weaken (Tele.nil : Ctx n n) = Tele.nil := rfl
+theorem weaken_nil {n} : weaken (Tele.nil : Ctx n n) = Tele.nil := rfl
 
-theorem Ctx.weaken_snoc {m n src x A}
+theorem weaken_snoc {m n src x A}
     (Γ : Ctx m n) :
-    Ctx.weaken (Γ.snoc ⟨src, x, A⟩) = Nat.succ_add n 1 ▸ (Ctx.weaken Γ).snoc ⟨src, x, A.weaken⟩ := by
-  unfold Ctx.weaken
+    weaken (Γ.snoc ⟨src, x, A⟩) = Nat.succ_add n 1 ▸ (weaken Γ).snoc ⟨src, x, A.weaken⟩ := by
+  unfold weaken
   rw [Tele.dmap_snoc]
 
 /-- Apply a single-variable substitution to a context -/
-def Ctx.subst {m} (a : Tm m) : {n : Nat} → Ctx (m + 1) (n + 1) → Ctx m n
+def subst {m} (a : Tm m) : {n : Nat} → Ctx (m + 1) (n + 1) → Ctx m n
   | _, .nil => .nil
   | n + 1, .snoc Γ ⟨src, x, B⟩ =>
       have := Γ.le
       have heq : m + (n - m) = n := by omega
-      .snoc (Ctx.subst a Γ) ⟨src, x, B.subst (Subst.beta (heq ▸ a.subst (Subst.shiftN (n - m))))⟩
+      .snoc (subst a Γ) ⟨src, x, B.subst (Subst.beta (heq ▸ a.subst (Subst.shiftN (n - m))))⟩
 
 instance {m n} : GetElem (Ctx (m + 1) (n + 1)) (Tm m) (Ctx m n) fun _ _ => True where
-  getElem Γ s _ := Ctx.subst s Γ
+  getElem Γ s _ := subst s Γ
 
 @[simp]
-theorem Ctx.subst_nil {n} {a : Tm n} : Ctx.subst a Tele.nil = Tele.nil := by
-  unfold Ctx.subst
+theorem subst_nil {n} {a : Tm n} : subst a Tele.nil = Tele.nil := by
+  unfold subst
   rfl
+
+end Ctx
 
 end Qdt
